AwsCryptographicMaterialProviders/dafny/AwsCryptographyKeyStoreAdmin/src/AwsCryptographyKeyStoreAdminOperations.dfy
@@ -8,6 +8,7 @@ include "KmsUtils.dfy"
 include "DescribeMutation.dfy"
 include "CreateKeysHV2.dfy"
 include "BKSAOperationUtils.dfy"
+include "KeyStoreAdminErrorMessages.dfy"
 
 module AwsCryptographyKeyStoreAdminOperations refines AbstractAwsCryptographyKeyStoreAdminOperations {
   import opened AwsKmsUtils
@@ -33,6 +34,7 @@ module AwsCryptographyKeyStoreAdminOperations refines AbstractAwsCryptographyKey
   import KmsUtils
   import CreateKeysHV2
   import OptUtils = BKSAOperationUtils
+  import KeyStoreAdminErrorMessages
 
   datatype Config = Config(
     nameonly logicalKeyStoreName: string,
@@ -456,8 +458,11 @@ module AwsCryptographyKeyStoreAdminOperations refines AbstractAwsCryptographyKey
     assume {:axiom} keyManagerStrat.Modifies !! systemKey.Modifies;
 
     :- Need(
-      keyManagerStrat.SupportHV1(),
-      Types.KeyStoreAdminException(message := "At this time, Mutations do not support KeyManagementStrategy#AwsKmsSimple.")
+      !input.Mutations.TerminalHierarchyVersion.Some? || KmsUtils.IsSupportedKeyManagerStrategy(input.Mutations.TerminalHierarchyVersion.value, keyManagerStrat),
+      Types.UnsupportedFeatureException(
+        message :=
+          KeyStoreAdminErrorMessages.UNSUPPORTED_KEY_MANAGEMENT_STRATEGY
+      )
     );
     var internalInput := KSAInitializeMutation.InternalInitializeMutationInput(
       Identifier := input.Identifier,
@@ -486,10 +491,6 @@ module AwsCryptographyKeyStoreAdminOperations refines AbstractAwsCryptographyKey
     assume {:axiom} keyManagerStrat.Modifies < MutationLie();
     assume {:axiom} keyManagerStrat.Modifies !! systemKey.Modifies;
 
-    :- Need(
-      keyManagerStrat.SupportHV1(),
-      Types.KeyStoreAdminException(message := "At this time, Mutations do not support KeyManagementStrategy#AwsKmsSimple.")
-    );
     var internalInput := KSAApplyMutation.InternalApplyMutationInput(
       MutationToken := input.MutationToken,
       PageSize := input.PageSize,
